
\(\)
\paragraph{The specified dynamical system}
\(
\)\par

\(\dot u_{1}=\pi  u\sb2
\)\par

\(\dot u_{2}=-\pi  u\sb1+\pi ^{-1} \eps u\sb1 u\sb5
\)\par

\(\dot u_{3}=\pi  u\sb4
\)\par

\(\dot u_{4}=-\pi  u\sb3+\pi ^{-1} \eps u\sb3 u\sb5
\)\par

\(\dot u_{5}=2 \pi  u\sb6
\)\par

\(\dot u_{6}=-2 \pi  u\sb5+\pi ^{-1} \eps \big(1/2 u\sb1^{2}+1/2 u\sb3^{2}
\big)
\)\par

\(\)
\paragraph{Invariant subspace basis vectors}
\(
\)\par

\(\vec e_{1}=\left\{
\left\{
1 , i , 0 , 0 , 0 , 0
\right\} , \exp \big(i \pi  t\big)
\right\}
\)\par

\(\vec e_{2}=\left\{
\left\{
1 , -i , 0 , 0 , 0 , 0
\right\} , \exp \big(-i \pi  t\big)
\right\}
\)\par

\(\vec e_{3}=\left\{
\left\{
0 , 0 , 1 , i , 0 , 0
\right\} , \exp \big(i \pi  t\big)
\right\}
\)\par

\(\vec e_{4}=\left\{
\left\{
0 , 0 , 1 , -i , 0 , 0
\right\} , \exp \big(-i \pi  t\big)
\right\}
\)\par

\(\vec e_{5}=\left\{
\left\{
0 , 0 , 0 , 0 , 1 , i
\right\} , \exp \big(2 i \pi  t\big)
\right\}
\)\par

\(\vec e_{6}=\left\{
\left\{
0 , 0 , 0 , 0 , 1 , -i
\right\} , \exp \big(-2 i \pi  t\big)
\right\}
\)\par

\(\vec z_{1}=\left\{
\left\{
1/2 , 1/2 i , 0 , 0 , 0 , 0
\right\} , \exp \big(i \pi  t\big)
\right\}
\)\par

\(\vec z_{2}=\left\{
\left\{
1/2 , -1/2 i , 0 , 0 , 0 , 0
\right\} , \exp \big(-i \pi  t\big)
\right\}
\)\par

\(\vec z_{3}=\left\{
\left\{
0 , 0 , 1/2 , 1/2 i , 0 , 0
\right\} , \exp \big(i \pi  t\big)
\right\}
\)\par

\(\vec z_{4}=\left\{
\left\{
0 , 0 , 1/2 , -1/2 i , 0 , 0
\right\} , \exp \big(-i \pi  t\big)
\right\}
\)\par

\(\vec z_{5}=\left\{
\left\{
0 , 0 , 0 , 0 , 1/2 , 1/2 i
\right\} , \exp \big(2 i \pi  t\big)
\right\}
\)\par

\(\vec z_{6}=\left\{
\left\{
0 , 0 , 0 , 0 , 1/2 , -1/2 i
\right\} , \exp \big(-2 i \pi  t\big)
\right\}
\)\par
