\documentclass[11pt,a5paper]{article}
\usepackage[a5paper,margin=13mm]{geometry}
\usepackage{parskip,time} \raggedright
\def\cis\big(#1\big){\,e^{#1i}}
\def\eps{\varepsilon}
\title{Centre manifold of your dynamical system}
\author{A. J. Roberts, University of Adelaide\\
\texttt{http://www.maths.adelaide.edu.au/anthony.roberts}}
\date{\now, \today}
\begin{document}
\maketitle
Throughout and generally: the lowest order, most
important, terms are near the end of each expression.
\input{centreManSys}

\(
\)
\paragraph{The centre manifold}
These give the location of the centre manifold in
terms of parameters~\(s\sb j\).
\(
\)\par

\(u_{1}=s_{1}
\)\par

\(u_{2}=s_{2}
\)\par

\(u_{3}=s_{3}
\)\par

\(u_{4}=-b \eps s_{2} s_{1}
\)\par

\(u_{5}=b \eps^{2} \big(-s_{3} s_{2}^{2}+s_{3} s_{1}^{2}\big)
\)\par

\(
\)
\paragraph{Centre manifold ODEs}
The system evolves on the centre manifold such
that the parameters evolve according to these ODEs.
\(
\)\par

\(\dot s_{1}=b^{2} \eps^{3} \big(-s_{3} s_{2}^{3}+s_{3} s_{2} s_{1}^{2}
\big)-\eps s_{3} s_{2}
\)\par

\(\dot s_{2}=b^{2} \eps^{3} \big(s_{3} s_{2}^{2} s_{1}-s_{3} s_{1}^{3}
\big)+\eps s_{3} s_{1}
\)\par

\(\dot s_{3}=-\eps s_{2} s_{1}
\)\par

\(
\)
\paragraph{Normals to isochrons at the slow manifold}
Use these vectors: to project initial conditions
onto the slow manifold; to project non-autonomous
forcing onto the slow evolution; to predict the
consequences of modifying the original system; in
uncertainty quantification to quantify effects on
the model of uncertainties in the original system.
The normal vector \(\vec z\sb j:=(z\sb{j1},\ldots,z\sb{jn}\
)\)
\(
\)\par

\(z_{11}=b^{2} \eps^{2} s_{2}^{2}+1
\)\par

\(z_{12}=b^{2} \eps^{2} s_{2} s_{1}
\)\par

\(z_{13}=0
\)\par

\(z_{14}=b^{3} \eps^{3} \big(s_{2}^{3}-s_{2} s_{1}^{2}\big)+b \eps^{3} 
\big(-s_{2}^{3}+s_{2} s_{1}^{2}\big)+b \eps s_{2}
\)\par

\(z_{15}=0
\)\par

\(z_{21}=-b^{2} \eps^{2} s_{2} s_{1}
\)\par

\(z_{22}=-b^{2} \eps^{2} s_{1}^{2}+1
\)\par

\(z_{23}=0
\)\par

\(z_{24}=b^{3} \eps^{3} \big(-s_{2}^{2} s_{1}+s_{1}^{3}\big)+b \eps^{3} 
\big(s_{2}^{2} s_{1}-s_{1}^{3}\big)-b \eps s_{1}
\)\par

\(z_{25}=0
\)\par

\(z_{31}=0
\)\par

\(z_{32}=0
\)\par

\(z_{33}=1
\)\par

\(z_{34}=-4 b \eps^{3} s_{3} s_{2} s_{1}
\)\par

\(z_{35}=b \eps^{2} \big(-s_{2}^{2}+s_{1}^{2}\big)
\)\par
\end{document}
